examples/map/MapMAproof.v
@@ -1,6 +1,7 @@
 Require Import CRIS.
 
 Require Import MapHeader MapM MapA.
+Require Import wpsim_tactics ltac2_lib.
 
 Set Implicit Arguments.
 
@@ -9,6 +10,13 @@ Local Open Scope nat_scope.
 Module MapMA. Section MapMA.
   Import MapAS.
   Context `{!invG α Σ Γ, !subHG Γ Σ, !sinvG Σ Γ α β τ, !MapAGΓ Γ, !MapMGΓ Γ}.
+  Context `{ModRel υ ν, n : level}.
+
+  Context (ginv_s : invspec) (Spc_s : string → option fspec).
+  Context (MapInSpcS : spc_incl (MapAS.Spc υ n) Spc_s).
+
+  Context (ginv_t : invspec) (Spc_t : string → option fspec).
+  Context (MapInSpcT : spc_incl (MapMS.Spc ν n) Spc_t).
 
   Definition Ist : nat → alist key Any.t → alist key Any.t → iProp Σ :=
     (λ _ st_src st_tgt,
@@ -21,147 +29,141 @@ Module MapMA. Section MapMA.
             ∗ auth_allocated f
             ∗ auth_unallocated sz))%I.
 
-  Variable ginvH : invspec.
-  Variable SpcH : string → option fspec.
-  Hypothesis MapInSpcH : spc_incl MapAS.Spc SpcH.
+  Local Notation MapA := (MapA.t υ n ginv_s Spc_s ).
+  Local Notation MapM := (MapM.t ν n ginv_t Spc_t ).
 
-  Variable ginvL : invspec.
-  Variable SpcL : string → option fspec.
-  Hypothesis MapInSpcL : spc_incl MapMS.Spc SpcL.
-
-  Local Notation MapA := (MapA.t ginvH SpcH).
-  Local Notation MapM := (MapM.t ginvL SpcL).
-  
   Lemma simF_init : HSim.sim_fun open MapA MapM Ist MapName.init.
   Proof.
-    init_simF.
+    init_wpsim.
+    iDestruct "ASM" as "[[[-> %range] P] ->]".
 
     (* SRC: handle the IST of Map and the precond of init *)
-    steps_l. iDestruct "ASM" as "((% & P) & %)".
     iDestruct "IST" as (f sz) "(% & [(% & P0 & INIT) | (P' & B & U)])"; cycle 1.
     { iExFalso. iApply (pending_unique with "P P'"). }
     des. hss. rename q into sz.
     
     (* TGT: prove the precond of init *)
-    step_r. forces_r. iSplitL "P0". { iFrame. eauto. }
+    w_step_r. w_force_r sz. w_force_r ([Vint sz] ↑). w_force_r.
+    iSplitL "P0". { iFrame. eauto. }
 
     (* TGT: handle the postcond of init *)
-    hss. steps_r. iDestruct "GRT" as "(_ & %)". hss.
+    hss. w_steps_r. iDestruct "GRT" as "(_ & %)". hss.
     
     (* SRC: prove the postcond of init *)
     iMod (initialize with "INIT") as "(ALLOC & UNALLOC & INIT)".
-    forces_l. steps_l. forces_l.
+    w_force_l. w_steps_l. w_force_l. w_force_l.
     iSplitL "INIT". { iFrame. eauto. }
     
     (* prove the IST of Map *)
-    step. iSplit; eauto.
+    w_step. iSplit; eauto.
     iExists _, _. iSplitR; eauto. iRight. iFrame. 
   Qed.
 
   Lemma simF_get : HSim.sim_fun open MapA MapM Ist MapName.get.
   Proof.
-    init_simF.
+    init_wpsim.
+    destruct q as [k v]; s.
+    iDestruct "ASM" as "((-> & MAP) & ->)".
 
     (* SRC: handle the IST of Map and the precond of get *)
-    steps_l. iDestruct "ASM" as "((% & MAP) & %)".
     iDestruct "IST" as (f sz) "(% & [(% & P0 & INIT)|(P' & B & U)])".
     { iExFalso. iApply (initial_map_points_to with "INIT MAP"). }
-    des. hss. steps_l.
-    rename q1 into idx, q2 into v.
+    hss. w_steps_l. hss. w_steps_l.
 
     (* TGT: prove the precond of get *)
-    step_r. forces_r. hss. iSplit. { iFrame. eauto. }
+    w_step_r. w_force_r k. w_force_r. w_force_r.
+    iSplit; first eauto.
 
     (* TGT : handle the body of get *)
-    steps_r. hss. steps_r.
+    hss. w_steps_r. hss. w_steps_r.
     iPoseProof (auth_unallocated_points_to with "U MAP") as "%".
-    forces_r; eauto.
+    w_force_r.
 
     (* TGT: handle the postcond of get *)
-    steps_r. hss. steps_r. iDestruct "GRT" as "(_ & %)". subst.
+    w_steps_r. hss. w_steps_r. iDestruct "GRT" as "(_ & <-)".
 
     (* SRC: prove the postcond of get *)
-    steps_l. forces_l.
-    iPoseProof (auth_allocated_get with "B MAP") as "%". subst.
+    w_force_l. w_force_l.
+    iPoseProof (auth_allocated_get with "B MAP") as "->".
     iSplitL "MAP". { iFrame. eauto. }
 
     (* prove the IST of Map *)
-    step. iSplit; eauto.
+    w_step. iSplit; eauto.
     iExists _, _. iSplit; eauto. iRight. iFrame.
   Unshelve. lia.
   Qed.
 
   Lemma simF_set : HSim.sim_fun open MapA MapM Ist MapName.set.
   Proof.
-    init_simF.
+    init_wpsim.
 
     (* SRC: handle the IST of Map and the precond of set *)
-    steps_l. iDestruct "ASM" as "((% & MAP) & %)".
+    destruct q as [[k w] v].
+    iDestruct "ASM" as "((-> & MAP) & ->)".
     iDestruct "IST" as (f sz) "(% & [(% & P0 & INIT)|(P' & B & U)])".
     { iExFalso. iApply (initial_map_points_to with "INIT MAP"). }
-    des. hss. steps_l. hss. steps_l.
-    rename q2 into v', q3 into idx, q4 into v. hss.
+    des. hss. w_steps_l. hss. w_steps_l. hss.
 
     (* TGT: prove the precond of set *)
-    step_r. force_r (idx,v'). forces_r. iSplitR; first eauto.
+    w_step_r. w_force_r (k, v). w_force_r. w_force_r. iSplitR; first eauto.
 
     (* TGT : handle the body of set *)
-    hss. steps_r. hss. steps_r.
+    hss. w_steps_r. hss. w_steps_r.
     iPoseProof (auth_unallocated_points_to with "U MAP") as "%".
-    forces_r; eauto.
+    w_force_r. w_steps_r. hss. w_steps_r.
 
     (* TGT: handle the postcond of set *)
-    steps_r. hss. steps_r. iDestruct "GRT" as "(_ & %)". hss.
+    iDestruct "GRT" as "(_ & <-)".
     
     (* SRC : prove the postcond of set *)
     iPoseProof (auth_allocated_set with "B MAP") as ">(B & MAP)".
-    forces_l. iSplitL "MAP". { iFrame. eauto. }
+    w_force_l. w_force_l. iSplitL "MAP". { iFrame. eauto. }
 
     (* prove the IST of Map *)
-    step. iSplit; eauto.
+    w_step. iSplit; eauto.
     iExists _, _. iSplit; eauto. iRight. iFrame.
   Unshelve. done.
   Qed.
 
   Lemma simF_set_by_user : HSim.sim_fun open MapA MapM Ist MapName.set_by_user.
   Proof.
-    init_simF.
+    init_wpsim.
 
     (* SRC: handle the IST of Map and the precond of set_by_user *)
-    steps_l. iDestruct "ASM" as "((% & MAP) & %)".
-    hss. steps_l.
-    rename q1 into idx, q2 into v.
-    
+    destruct q as [k w].
+    iDestruct "ASM" as "((-> & MAP) & ->)".
+    hss. w_steps_l.
+
     (* TGT: prove the precond of set_by_user *)
-    step_r. forces_r. hss. iSplitR. { eauto. }
+    w_step_r. w_force_r. w_force_r. w_force_r. hss. iSplitR. { eauto. }
 
     (* process an input *)
-    steps_r. step.
+    w_steps_r. w_step.
 
     (* TGT: handle the precond of set *)
-    steps_r. iDestruct "GRT" as "%". des. hss.
+    w_steps_r. iDestruct "GRT" as "%". des. hss.
     
     (* SRC: prove the precond of set *)
-    steps_l. force_l (_,_,_). forces_l.
+    w_steps_l. w_force_l (_,_,_). w_force_l. w_force_l.
     iSplitL "MAP". { iFrame. eauto. }
 
     (* make a call to set *)
-    call "IST". { eauto. }
+    w_call "IST".
 
     (* SRC: handle the postcond of set *)
-    steps_l. iDestruct "ASM" as "((% & MAP) & %)". hss.
+    w_steps_l. iDestruct "ASM" as "((-> & MAP) & ->)". hss.
 
     (* TGT: prove the postcond of set *)
-    steps_l. forces_r. iSplitR. { iFrame. eauto. }
+    w_steps_l. w_force_r. w_force_r. iSplitR. { iFrame. eauto. }
 
     (* TGT: handle the postcond of set_by_user *)
-    steps_r. hss. steps_r. iDestruct "GRT" as "(_ & %)". subst.
+    w_steps_r. hss. w_steps_r. iDestruct "GRT" as "(_ & <-)".
     
     (* SRC: prove the postcond of set_by_user *)
-    forces_l. iSplitL "MAP". { iFrame. eauto. }
+    w_force_l. w_force_l. iSplitL "MAP". { iFrame. eauto. }
 
     (* prove the IST of Map *)
-    step. eauto.
+    w_step. eauto.
   Qed.
 
   Theorem sim : HSim.t open MapA MapM MapA.InitCond Ist.
