theories/simulations/wpsim/wpsim_tactics.v
@@ -94,101 +94,8 @@ Ltac _w_step_l :=
       match goal with [ H: ?x = Some _ |- _ ] => let G := fresh "G" in rename H into G; try rewrite -> G in * end
   end.
 
-Ltac _w_step_r :=
-  match goal with
-  (******* isim ******)
-  (** tgt **)
-  | [ |- environments.envs_entails _ (wpsim _ _ _ _ _ _ _ _ _ _ _ _ _ _ _ _ _ _ (_, tau;; _)) ] =>
-      iApply wpsim_tau_tgt
-  | [ |- environments.envs_entails _ (wpsim _ _ _ _ _ _ _ _ _ _ _ _ _ _ _ _ _ _ (_, Ret _ >>= _) ) ] =>
-      rewrite bind_ret_l
-  | [ |- environments.envs_entails _ (wpsim _ _ _ _ _ _ _ _ _ _ _ _ _ _ _ _ _ _ (_, trigger (Choose _) >>= _) ) ] =>
-      let name := fresh "q" in iApply wpsim_choose_tgt; iIntros (name)
-  | [ |- environments.envs_entails _ (wpsim _ _ _ _ _ _ _ _ _ _ _ _ _ _ _ _ _ _ (_, trigger (Guarantee ?P) >>= _) ) ] =>
-      unfold_precond_postcond P; iApply wpsim_guarantee_tgt; iIntrosFresh "GRT"
-  | [ |- environments.envs_entails _ (wpsim _ _ _ _ _ _ _ _ _ _ _ _ _ _ _ _ _ _ (_, guarantee _ >>= _)) ] =>
-      let name := fresh "grt" in iApply wpsim_guar_tgt; iIntros (name)
-  | [ |- environments.envs_entails _ (wpsim _ _ _ _ _ _ _ _ _ _ _ _ _ _ _ _ _ _ (_, (HMod.sandbox _ (trigger (SPut _ _))) >>= _)) ] =>
-      iApply wpsim_sput_tgt_sandbox; [s; eauto|]
-  | [ |- environments.envs_entails _ (wpsim _ _ _ _ _ _ _ _ _ _ _ _ _ _ _ _ _ _ (_, (HMod.sandbox _ (trigger (SGet _))) >>= _)) ] =>
-      iApply wpsim_sget_tgt_sandbox; [s; eauto|]
-  (* 
-  | [ |- environments.envs_entails _ (isim _ _ _ _ _ _ _ _ _ _ _ _ (_, unwrapN ?ox >>= _)) ] =>
-      let name := fresh "q" in
-      iApply isim_unwrapN_tgt; iIntros (name) "%";
-      match goal with [ H: ?x = Some _ |- _ ] => let G := fresh "G" in rename H into G; try rewrite -> G in * end
-*)
-  | [ |- environments.envs_entails _ (wpsim _ _ _ _ _ _ _ _ _ _ _ _ _ _ _ _ _ _ (_, trigger Tid >>= _)) ] =>
-      iApply wpsim_tid_tgt
-  end.
-
 Ltac w_step_l_core :=
   _w_step_l; try alist_find_simpl; s; des_pairs; s.
-Ltac w_step_r_core :=
-  _w_step_r; try alist_find_simpl; s; des_pairs; s.
-
-Ltac _w_force_l :=
-  match goal with
-  | [ |- environments.envs_entails _ (wpsim _ _ _ _ _ _ _ _ _ _ _ _ _ _ _ _ _ (_, trigger (Choose ?T) >>= _) _) ] =>
-      iApply wpsim_choose_src
-  | [ |- environments.envs_entails _ (wpsim _ _ _ _ _ ?υ _ ?n _ _ _ _ _ _ _ _ _ (_, trigger (Guarantee ?P) >>= _) _) ] =>
-      first [
-        tcsearch constr:(WP P υ n ⊤)
-          ltac:(fun c =>
-            iApply (wpsim_full_guarantee_src_WP _ _ _ _ _ _ _ _ _ _ _ _ _ _ _ _ _ _ _ (i:=c)); simpl);
-        match goal with
-        | [ |- environments.envs_entails _ (?P' ∗ _)] =>
-          unfold_precond_postcond P'
-        end
-      | unfold_precond_postcond P; iApply wpsim_guarantee_src
-      ]
-  | [ |- environments.envs_entails _ (wpsim _ _ _ _ _ _ _ _ _ _ _ _ _ _ _ _ _ (_, unwrapN _ >>= _) _) ] =>
-      iApply wpsim_unwrapN_src
-  (* | [ |- environments.envs_entails _ (isim _ _ _ _ _ _ _ _ _ _ _ (_, guarantee _ >>= _) _) ] =>
-      iApply isim_guar_src *)
-  end.
-
-(* Ltac preprocess_l tac :=
-  let marker := fresh "MARKER" in
-  set_marker marker;
-  hide_ihyps;
-  hide_itree_r;
-  prep;
-  tac;
-  show_until marker.
-
-Ltac preprocess_r tac :=
-  let marker := fresh "MARKER" in
-  set_marker marker;
-  hide_ihyps;
-  hide_itree_l;
-  prep;
-  tac;
-  show_until marker.
-
-Ltac preprocess_both tac :=
-  let marker := fresh "MARKER" in
-  set_marker marker;
-  hide_ihyps;
-  hide_itree_l; prep; show_itree;
-  hide_itree_r; prep; show_itree;
-  tac;
-  show_until marker.
-   *)
-Ltac w_force_l_core :=
-  let marker := fresh "MARKER" in
-  set_marker marker;
-  hide_ihyps;
-  hide_itree_r;
-  prep;
-  _w_force_l;
-  show_until marker.
-
-Tactic Notation "w_force_l" :=
-  w_force_l_core; try (iExists _).
-
-Tactic Notation "w_force_l" uconstr(p) :=
-  w_force_l_core; iExists p.
 
 Ltac w_step :=
   let marker := fresh "MARKER" in
@@ -216,6 +123,46 @@ Ltac w_steps_l :=
   (hrepeat do 1 (prep; w_step_l_core));
   show_until marker.
 
+Ltac _w_step_r :=
+  match goal with
+  (******* isim ******)
+  (** tgt **)
+  | [ |- environments.envs_entails _ (wpsim _ _ _ _ _ _ _ _ _ _ _ _ _ _ _ _ _ _ (_, tau;; _)) ] =>
+      iApply wpsim_tau_tgt
+  | [ |- environments.envs_entails _ (wpsim _ _ _ _ _ _ _ _ _ _ _ _ _ _ _ _ _ _ (_, Ret _ >>= _) ) ] =>
+      rewrite bind_ret_l
+  | [ |- environments.envs_entails _ (wpsim _ _ _ _ _ _ _ _ _ _ _ _ _ _ _ _ _ _ (_, trigger (Choose _) >>= _) ) ] =>
+      let name := fresh "q" in iApply wpsim_choose_tgt; iIntros (name)
+  | [ |- environments.envs_entails _ (wpsim _ _ _ _ _ _ ?ν ?n _ _ _ _ _ _ _ _ _ _ (_, trigger (Guarantee ?P) >>= _) ) ] =>
+      first [
+        tcsearch constr:(WP P ν n ⊤)
+          ltac:(fun c =>
+            iApply (wpsim_half_guarantee_tgt_WP _ _ _ _ _ _ _ _ _ _ _ _ _ _ _ _ _ _ _ (i:=c)); simpl);
+        match goal with
+        | [ |- environments.envs_entails _ (?P' -∗ _)] =>
+          unfold_precond_postcond P'; iIntrosFresh "GRT"
+        end
+      | unfold_precond_postcond P; iApply wpsim_guarantee_tgt; iIntrosFresh "GRT"
+      ]
+  | [ |- environments.envs_entails _ (wpsim _ _ _ _ _ _ _ _ _ _ _ _ _ _ _ _ _ _ (_, guarantee _ >>= _)) ] =>
+      let name := fresh "grt" in iApply wpsim_guar_tgt; iIntros (name)
+  | [ |- environments.envs_entails _ (wpsim _ _ _ _ _ _ _ _ _ _ _ _ _ _ _ _ _ _ (_, (HMod.sandbox _ (trigger (SPut _ _))) >>= _)) ] =>
+      iApply wpsim_sput_tgt_sandbox; [s; eauto|]
+  | [ |- environments.envs_entails _ (wpsim _ _ _ _ _ _ _ _ _ _ _ _ _ _ _ _ _ _ (_, (HMod.sandbox _ (trigger (SGet _))) >>= _)) ] =>
+      iApply wpsim_sget_tgt_sandbox; [s; eauto|]
+  (* 
+  | [ |- environments.envs_entails _ (isim _ _ _ _ _ _ _ _ _ _ _ _ (_, unwrapN ?ox >>= _)) ] =>
+      let name := fresh "q" in
+      iApply isim_unwrapN_tgt; iIntros (name) "%";
+      match goal with [ H: ?x = Some _ |- _ ] => let G := fresh "G" in rename H into G; try rewrite -> G in * end
+*)
+  | [ |- environments.envs_entails _ (wpsim _ _ _ _ _ _ _ _ _ _ _ _ _ _ _ _ _ _ (_, trigger Tid >>= _)) ] =>
+      iApply wpsim_tid_tgt
+  end.
+
+Ltac w_step_r_core :=
+  _w_step_r; try alist_find_simpl; s; des_pairs; s.
+
 Ltac w_step_r :=
   let marker := fresh "MARKER" in
   set_marker marker;
@@ -231,6 +178,99 @@ Ltac w_steps_r :=
   hide_ihyps;
   hide_itree_l;
   (hrepeat do 1 (prep; w_step_r_core));
+  show_until marker.
+
+Ltac _w_force_l :=
+  match goal with
+  | [ |- environments.envs_entails _ (wpsim _ _ _ _ _ _ _ _ _ _ _ _ _ _ _ _ _ (_, trigger (Choose ?T) >>= _) _) ] =>
+      iApply wpsim_choose_src
+  | [ |- environments.envs_entails _ (wpsim _ _ _ _ _ ?υ _ ?n _ _ _ _ _ _ _ _ _ (_, trigger (Guarantee ?P) >>= _) _) ] =>
+      first [
+        tcsearch constr:(WP P υ n ⊤)
+          ltac:(fun c =>
+            iApply (wpsim_full_guarantee_src_WP _ _ _ _ _ _ _ _ _ _ _ _ _ _ _ _ _ _ _ (i:=c)); simpl);
+        match goal with
+        | [ |- environments.envs_entails _ (?P' ∗ _)] =>
+          unfold_precond_postcond P'
+        end
+      | unfold_precond_postcond P; iApply wpsim_guarantee_src
+      ]
+  | [ |- environments.envs_entails _ (wpsim _ _ _ _ _ _ _ _ _ _ _ _ _ _ _ _ _ (_, unwrapN _ >>= _) _) ] =>
+      iApply wpsim_unwrapN_src
+  (* | [ |- environments.envs_entails _ (isim _ _ _ _ _ _ _ _ _ _ _ (_, guarantee _ >>= _) _) ] =>
+      iApply isim_guar_src *)
+  end.
+
+Ltac w_force_l_core :=
+  let marker := fresh "MARKER" in
+  set_marker marker;
+  hide_ihyps;
+  hide_itree_r;
+  prep;
+  _w_force_l;
+  show_until marker.
+
+Tactic Notation "w_force_l" :=
+  w_force_l_core; try (iExists _).
+
+Tactic Notation "w_force_l" uconstr(p) :=
+  w_force_l_core; iExists p.
+
+Ltac _w_force_r :=
+  match goal with
+  | [ |- environments.envs_entails _ (wpsim _ _ _ _ _ _ _ _ _ _ _ _ _ _ _ _ _ _ (_, trigger (Take _) >>= _)) ] =>
+      iApply wpsim_take_tgt
+  | [ |- environments.envs_entails _ (wpsim _ _ _ _ _ _ ?ν ?n _ _ _ _ _ _ _ _ _ _ (_, trigger (Assume ?P) >>= _)) ] =>
+      first [
+        tcsearch constr:(WP P ν n ⊤)
+          ltac:(fun c =>
+            iApply (wpsim_half_assume_tgt_WP _ _ _ _ _ _ _ _ _ _ _ _ _ _ _ _ _ _ _ (i:=c)); simpl);
+        match goal with
+        | [ |- environments.envs_entails _ (?P' ∗ _)] =>
+          unfold_precond_postcond P'
+        end
+      | unfold_precond_postcond P; iApply wpsim_assume_tgt
+      ]
+  (* | [ |- environments.envs_entails _ (isim _ _ _ _ _ _ _ _ _ _ _ _ (_, unwrapU _ >>= _)) ] =>
+      iApply isim_unwrapU_tgt; iExists _
+  | [ |- environments.envs_entails _ (isim _ _ _ _ _ _ _ _ _ _ _ _ (_, assume _ >>= _)) ] =>
+      iApply isim_asm_tgt *)
+  end
+.
+
+Ltac w_force_r_core :=
+  let marker := fresh "MARKER" in
+  set_marker marker;  
+  hide_ihyps;
+  hide_itree_l;
+  prep;
+  _w_force_r; s;
+  show_until marker.
+
+Tactic Notation "w_force_r" :=
+  w_force_r_core; try (iExists _).
+
+Tactic Notation "w_force_r" uconstr(p) :=
+  w_force_r_core; iExists p.
+
+Ltac w_inline_l :=
+  let marker := fresh "MARKER" in
+  set_marker marker;  
+  hide_ihyps;
+  hide_itree_r;
+  prep;
+  iApply wpsim_inline_src; [prove_inline_cond|];
+  unfold_cris_defs;
+  show_until marker.
+
+Ltac w_inline_r :=
+  let marker := fresh "MARKER" in
+  set_marker marker;  
+  hide_ihyps;
+  hide_itree_l;
+  prep;
+  iApply wpsim_inline_tgt; [prove_inline_cond|];
+  unfold_cris_defs;
   show_until marker.
 
 Ltac by_coind CIH :=
